memmove

bedrock2/src/bedrock2Examples/memmove.v
@@ -6,6 +6,9 @@ Local Open Scope string_scope. Local Open Scope Z_scope. Local Open Scope list_s
 Require Import bedrock2.WeakestPrecondition bedrock2.Semantics bedrock2.ProgramLogic.
 Require Import coqutil.Word.Interface coqutil.Word.Bitwidth.
 Require Import coqutil.Map.Interface bedrock2.Map.SeparationLogic.
+Require Import bedrock2.ZnWords.
+Import Coq.Init.Byte coqutil.Byte.
+Local Notation string := String.string.
 
 (*Require Import bedrock2.ptsto_bytes.*)
 Require Import coqutil.Map.OfListWord.
@@ -14,15 +17,382 @@ Local Notation "m =* P" := ((P%sep) m) (at level 70, only parsing) (* experiment
 
 Section WithParameters.
   Context {width} {BW: Bitwidth width}.
-  Context {word: word.word width} {mem: map.map word Byte.byte} {locals: map.map String.string word}.
+  Context {word: word.word width} {mem: map.map word byte} {locals: map.map string word}.
   Context {ext_spec: ExtSpec}.
-  Context {word_ok: word.ok word} {mem_ok: map.ok mem}.
   Import ProgramLogic.Coercions.
 
 
-  Instance spec_of_memmove : spec_of "memmove" :=
-    fnspec! "memmove" dst src (n : word) / d s R Rs,
+  Local Instance spec_of_memmove : spec_of "memmove" :=
+    fnspec! "memmove" (dst src n : word) / (d s : list byte) (R Rs : mem -> Prop),
     { requires t m := m =* s$@src * Rs /\ m =* d$@dst * R /\
-      length s = n :> Z /\ length d = n :> Z /\ n < 2^(width-1);
-      ensures t' m' := t=t' /\ sep (eq(s$@dst)) R m }.
+        length s = n :> Z /\ length d = n :> Z /\ n <= 2^(width-1);
+      ensures t' m := m =* s$@dst * R /\ t=t' }.
+
+
+  Definition memmove : Syntax.func :=
+    ("memmove", (["dst"; "src"; "n"], [], bedrock_func_body:(
+    x = src-dst;
+    require x;
+    if x < x+n {
+      while n {
+        store1(dst, load1(src));
+        src = src + $1;
+        dst = dst + $1;
+        n = n - $1
+      }
+    } else {
+      dst = dst + (n - $1);
+      src = src + (n - $1);
+      while n {
+        store1(dst, load1(src));
+        src = src - $1;
+        dst = dst - $1;
+        n = n - $1
+      }
+    }
+  ))).
+
+
+  Context {word_ok: word.ok word} {mem_ok: map.ok mem} {locals_ok : map.ok locals}
+    {env : map.map string (list string * list string * Syntax.cmd)} {env_ok : map.ok env}
+    {ext_spec_ok : ext_spec.ok ext_spec}.
+
+  Import coqutil.Tactics.letexists coqutil.Tactics.Tactics coqutil.Tactics.autoforward.
+  Require Import coqutil.Word.Properties coqutil.Map.Properties.
+
+  Local Ltac ZnWords := destruct width_cases; bedrock2.ZnWords.ZnWords.
+  Lemma memmove_ok : program_logic_goal_for_function! memmove.
+  Proof.
+    repeat straightline.
+
+    case H as (ms&mRs&?&?&?), H0 as (md&mRd&?&?&?);
+      cbv [sepclause_of_map] in *; subst; clear dependent Rs.
+
+    eapply WeakestPreconditionProperties.dexpr_expr.
+    repeat straightline.
+    letexists; split.
+    { subst l; rewrite ?Properties.map.get_put_dec; exact eq_refl. }
+    letexists; split.
+    { subst l; rewrite ?Properties.map.get_put_dec; exact eq_refl. }
+    repeat straightline.
+
+    set (x := word.sub src dst) in *.
+    unfold1_cmd_goal; cbv beta match delta [cmd_body].
+    eapply WeakestPreconditionProperties.dexpr_expr.
+    letexists; split.
+    { subst l0; rewrite ?Properties.map.get_put_dec; exact eq_refl. }
+    repeat straightline.
+
+    (* x = 0 *)
+    split; intros Hx; cycle 1.
+    { replace src with dst in * by ZnWords.
+      cbn; ssplit; eauto.
+      eexists _, _; ssplit; eauto.
+      eapply map.split_same_footprint; eauto.
+      intros k.
+      rewrite 2map.get_of_list_word_at, 2List.nth_error_None.
+      Morphisms.f_equiv. ZnWords. }
+
+    unfold1_cmd_goal; cbv beta match delta [cmd_body].
+    eapply WeakestPreconditionProperties.dexpr_expr.
+    letexists; split.
+    { subst l0; rewrite ?Properties.map.get_put_dec; exact eq_refl. }
+    repeat straightline.
+    letexists; split.
+    { subst l0; rewrite ?Properties.map.get_put_dec; exact eq_refl. }
+    letexists; split.
+    { subst l0 l; rewrite ?Properties.map.get_put_dec. exact eq_refl. }
+    repeat straightline.
+
+    rewrite word.unsigned_ltu, word.unsigned_add; cbv [word.wrap].
+    split; intros Hbr;
+      [apply word.if_nonzero in Hbr | apply word.if_zero in Hbr];
+      autoforward with typeclass_instances in Hbr.
+
+    { assert (x + n < 2^width) by ZnWords.
+      refine ((Loops.tailrec
+        (HList.polymorphic_list.cons _
+        (HList.polymorphic_list.cons _
+        (HList.polymorphic_list.cons _
+        (HList.polymorphic_list.cons _
+        HList.polymorphic_list.nil))))
+        ["dst";"src";"n";"x"])
+        (fun (v:nat) s mRs d mRd t m dst src n _x => PrimitivePair.pair.mk (
+          x + n < 2^width /\ map.split m (s$@src) mRs /\  map.split m (d$@dst) mRd /\
+          x = word.sub src dst /\ v=n :> Z /\ length s = n :> Z /\ length d = n :> Z
+        )
+        (fun                     T M DST SRC N X => t = T   /\  map.split M (s$@dst) mRd))
+        lt
+        _ _ _ _ _ _ _ _ _);
+        (* TODO wrap this into a tactic with the previous refine *)
+        cbn [HList.hlist.foralls HList.tuple.foralls
+             HList.hlist.existss HList.tuple.existss
+             HList.hlist.apply  HList.tuple.apply
+             HList.hlist
+             List.repeat Datatypes.length
+             HList.polymorphic_list.repeat HList.polymorphic_list.length
+             PrimitivePair.pair._1 PrimitivePair.pair._2] in *.
+        { cbv [Loops.enforce]; cbn.
+          subst l l0.
+          repeat (rewrite ?map.get_put_dec, ?map.get_remove_dec; cbn); split.
+          { exact eq_refl. }
+          { eapply map.map_ext; intros k.
+            repeat (rewrite ?map.get_put_dec, ?map.get_remove_dec, ?map.get_empty; cbn -[String.eqb]).
+            repeat (destruct String.eqb; trivial). } }
+        { eapply Wf_nat.lt_wf. }
+        { cbn; ssplit; eauto. }
+        { intros ?v ?s ?mRs ?d ?mRd ?t ?m ?dst ?src ?n ?x.
+          repeat straightline.
+          cbn in localsmap.
+          eexists n0; split; cbv [expr expr_body localsmap get].
+          { rewrite ?Properties.map.get_put_dec. exists n0; cbn. auto. }
+          split; cycle 1.
+          { intros Ht; rewrite Ht in *.
+            intuition idtac; destruct s0, d0; cbn in *; try discriminate; [].
+            eauto. }
+          repeat straightline.
+          eapply WeakestPreconditionProperties.dexpr_expr.
+          repeat straightline.
+          letexists; split.
+          { rewrite ?Properties.map.get_put_dec; exact eq_refl. }
+          eapply WeakestPreconditionProperties.dexpr_expr.
+          repeat straightline.
+          letexists; split.
+          { rewrite ?Properties.map.get_put_dec; cbn. exact eq_refl. }
+          repeat straightline.
+
+          cbv [WeakestPrecondition.load load load_Z]; cbn.
+          destruct s0 as [|b s0], d0 as [|B d0]; try (cbn in *; congruence); [].
+          exists (word.of_Z (byte.unsigned b)).
+          pose proof map.get_split src0 _ _ _ H6.
+          rewrite map.get_of_list_word_at in H14.
+          progress replace (Z.to_nat (word.sub src0 src0)) with O in H14 by ZnWords;
+            cbn in H14; case H14 as [[? ?]|[? ?]]; try discriminate.
+          rewrite H14. split. { rewrite LittleEndianList.le_combine_1. trivial. }
+
+          cbv [WeakestPrecondition.store load load_Z load_bytes store store_Z store_bytes unchecked_store_bytes LittleEndianList.le_split]; cbn.
+          pose proof map.get_split dst0 _ _ _ H8.
+          rewrite map.get_of_list_word_at in H16.
+          progress replace (Z.to_nat (word.sub dst0 dst0)) with O in H16 by ZnWords;
+            cbn in H16; case H16 as [[? ?]|[? ?]]; try discriminate.
+          eexists. rewrite H16. split.
+          { rewrite word.unsigned_of_Z, Scalars.wrap_byte_unsigned.
+            rewrite byte.of_Z_unsigned; trivial. }
+
+          eapply map.split_remove_put in H6; [|eapply H14].
+          eapply map.split_remove_put in H8; [|eapply H16].
+          rewrite map.remove_head_of_list_word_at_cons in H6,H8 by (cbn in *; ZnWords).
+          assert (map.split (map.put m0 dst0 b) (s0$@(word.add src0 (word.of_Z 1))) (map.put (map.put mRs0 src0 b) dst0 b)).
+          { eapply map.split_put_None; trivial.
+            rewrite map.get_of_list_word_at, List.nth_error_None.
+            cbn in *; ZnWords. }
+          assert (map.split (map.put m0 dst0 b) (d0$@(word.add dst0 (word.of_Z 1))) (map.put mRd0 dst0 b)).
+          { rewrite <-map.put_put_same with (m:=mRd0) (v1 := B).
+            eapply map.split_put_Some; rewrite ?map.get_put_same; eauto. }
+
+          cbv [get literal dlet.dlet].
+          repeat (rewrite ?map.get_put_dec, ?map.get_remove_dec; cbn).
+          eexists.
+          eexists.
+          { eauto. }
+          eexists.
+          repeat (rewrite ?map.get_put_dec, ?map.get_remove_dec; cbn).
+          eexists.
+          { eauto. }
+          eexists.
+          eexists.
+          { eauto. }
+          eexists _, _, _, _.
+          split.
+          { cbv [Loops.enforce]; cbn.
+            repeat (rewrite ?map.get_put_dec, ?map.get_remove_dec; cbn); split.
+            { exact eq_refl. }
+            { eapply map.map_ext; intros k.
+              repeat (rewrite ?map.get_put_dec, ?map.get_remove_dec, ?map.get_empty; cbn -[String.eqb]).
+              repeat (destruct String.eqb; trivial). } }
+          eexists _, _, _, _, (length s0); split; ssplit.
+          { ZnWords. }
+          { eassumption. }
+          { eassumption. }
+          { ZnWords. }
+          { cbn in *; ZnWords. }
+          { cbn in *; ZnWords. }
+          { cbn in *; ZnWords. }
+          split.
+          { cbn in *; ZnWords. }
+          intuition idtac; repeat straightline_cleanup.
+          eapply map.split_put_r2l in H22; trivial.
+          rewrite <-map.of_list_word_at_cons in H22. exact H22. }
+        { cbn. intuition idtac. eexists _, _; ssplit; eauto. } }
+
+    { assert (n <= x) by ZnWords.
+
+      unfold1_cmd_goal; cbv beta match delta [cmd_body].
+      eapply WeakestPreconditionProperties.dexpr_expr.
+      repeat straightline.
+      letexists; split.
+      { subst l0 l; rewrite ?Properties.map.get_put_dec; exact eq_refl. }
+      letexists; split.
+      { subst l0 l; rewrite ?Properties.map.get_put_dec; exact eq_refl. }
+      repeat straightline.
+
+      eapply WeakestPreconditionProperties.dexpr_expr.
+      repeat straightline.
+      letexists; split.
+      { subst l1 l0 l; rewrite ?Properties.map.get_put_dec; exact eq_refl. }
+      letexists; split.
+      { subst l1 l0 l; rewrite ?Properties.map.get_put_dec; exact eq_refl. }
+      repeat straightline.
+
+      refine ((Loops.tailrec
+        (HList.polymorphic_list.cons _
+        (HList.polymorphic_list.cons _
+        (HList.polymorphic_list.cons _
+        (HList.polymorphic_list.cons _
+        HList.polymorphic_list.nil))))
+        ["dst";"src";"n";"x"])
+        (fun (v:nat) s mRs d mRd t m dst src n _x => PrimitivePair.pair.mk (
+          n <= x /\ map.split m (s$@(word.sub src (word.sub n (word.of_Z 1)))) mRs /\ 
+                    map.split m (d$@(word.sub dst (word.sub n (word.of_Z 1)))) mRd /\
+          x = word.sub src dst /\ v=n :> Z /\ length s = n :> Z /\ length d = n :> Z
+        )
+        (fun                     T M DST SRC N X => t = T   /\  map.split M (s$@(word.sub dst (word.sub n (word.of_Z 1)))) mRd))
+        lt
+        _ _ _ _ _ _ _ _ _);
+        (* TODO wrap this into a tactic with the previous refine *)
+        cbn [HList.hlist.foralls HList.tuple.foralls
+             HList.hlist.existss HList.tuple.existss
+             HList.hlist.apply  HList.tuple.apply
+             HList.hlist
+             List.repeat Datatypes.length
+             HList.polymorphic_list.repeat HList.polymorphic_list.length
+             PrimitivePair.pair._1 PrimitivePair.pair._2] in *.
+        { cbv [Loops.enforce]; cbn.
+          subst l l0 l1 l2.
+          repeat (rewrite ?map.get_put_dec, ?map.get_remove_dec; cbn); split.
+          { exact eq_refl. }
+          { eapply map.map_ext; intros k.
+            repeat (rewrite ?map.get_put_dec, ?map.get_remove_dec, ?map.get_empty; cbn -[String.eqb]).
+            repeat (destruct String.eqb; trivial). } }
+        { eapply Wf_nat.lt_wf. }
+        { cbn. subst v0 v. rewrite !word.word_sub_add_l_same_r. ssplit; eauto. ZnWords. }
+        { intros ?v ?s ?mRs ?d ?mRd ?t ?m ?dst ?src ?n ?x.
+          repeat straightline.
+          cbn in localsmap.
+          eexists n0; split; cbv [expr expr_body localsmap get].
+          { rewrite ?Properties.map.get_put_dec. exists n0; cbn. auto. }
+          split; cycle 1.
+          { intros Ht; rewrite Ht in *.
+            intuition idtac; destruct s0, d0; cbn in *; try discriminate; [].
+            rewrite map.of_list_word_nil in *; trivial. }
+          repeat straightline.
+          eapply WeakestPreconditionProperties.dexpr_expr.
+          repeat straightline.
+          letexists; split.
+          { rewrite ?Properties.map.get_put_dec; exact eq_refl. }
+          eapply WeakestPreconditionProperties.dexpr_expr.
+          repeat straightline.
+          letexists; split.
+          { rewrite ?Properties.map.get_put_dec; cbn. exact eq_refl. }
+          repeat straightline.
+
+          cbv [WeakestPrecondition.load load load_Z]; cbn.
+          destruct (@List.exists_last _ s0) as (s0'&b&H's) in *.
+          { intro. subst. cbn in *. ZnWords. }
+          destruct (@List.exists_last _ d0) as (d0'&B&H'd) in *.
+          { intro. subst. cbn in *. ZnWords. }
+          subst s0 d0; rename s0' into s0; rename d0' into d0; rewrite List.app_length in *; cbn [List.length] in *.
+          exists (word.of_Z (byte.unsigned b)).
+          pose proof map.get_split src0 _ _ _ H6.
+          rewrite !map.get_of_list_word_at, !List.nth_error_app2 in H14 by ZnWords.
+          match goal with H : context[List.nth_error [_] ?i = None] |- _ =>
+              replace i with O in H by ZnWords; cbn [List.nth_error] in H end.
+          cbn in H14; case H14 as [[? ?]|[? ?]]; try discriminate.
+          rewrite H14. split. { rewrite LittleEndianList.le_combine_1. trivial. }
+
+          cbv [WeakestPrecondition.store load load_Z load_bytes store store_Z store_bytes unchecked_store_bytes LittleEndianList.le_split]; cbn.
+          pose proof map.get_split dst0 _ _ _ H8.
+          rewrite !map.get_of_list_word_at, !List.nth_error_app2 in H16 by ZnWords.
+          match goal with H : context[List.nth_error [_] ?i = None] |- _ =>
+              replace i with O in H by ZnWords; cbn [List.nth_error] in H end.
+          case H16 as [[? ?]|[? ?]]; try discriminate.
+          eexists. rewrite H16. split.
+          { rewrite word.unsigned_of_Z, Scalars.wrap_byte_unsigned.
+            rewrite byte.of_Z_unsigned; trivial. }
+
+          eapply map.split_remove_put in H6; [|eapply H14].
+          eapply map.split_remove_put in H8; [|eapply H16].
+          rewrite !map.remove_last_of_list_word_at_snoc in H6,H8 by ZnWords.
+          assert (map.split (map.put m0 dst0 b) (s0$@(word.sub src0 (word.sub n0 (word.of_Z 1)))) (map.put (map.put mRs0 src0 b) dst0 b)).
+          { eapply map.split_put_None; trivial.
+            rewrite map.get_of_list_word_at, List.nth_error_None.
+            cbn in *; ZnWords. }
+          assert (map.split (map.put m0 dst0 b) (d0$@(word.sub dst0 (word.sub n0 (word.of_Z 1)))) (map.put mRd0 dst0 b)).
+          { rewrite <-map.put_put_same with (m:=mRd0) (v1 := B).
+            eapply map.split_put_Some; rewrite ?map.get_put_same; eauto. }
+
+          cbv [get literal dlet.dlet].
+          repeat (rewrite ?map.get_put_dec, ?map.get_remove_dec; cbn).
+          eexists.
+          eexists.
+          { eauto. }
+          eexists.
+          repeat (rewrite ?map.get_put_dec, ?map.get_remove_dec; cbn).
+          eexists.
+          { eauto. }
+          eexists.
+          eexists.
+          { eauto. }
+          eexists _, _, _, _.
+          split.
+          { cbv [Loops.enforce]; cbn.
+            repeat (rewrite ?map.get_put_dec, ?map.get_remove_dec; cbn); split.
+            { exact eq_refl. }
+            { eapply map.map_ext; intros k.
+              repeat (rewrite ?map.get_put_dec, ?map.get_remove_dec, ?map.get_empty; cbn -[String.eqb]).
+              repeat (destruct String.eqb; trivial). } }
+          eexists _, _, _, _, (length s0); split; ssplit.
+          { ZnWords. }
+          { replace (word.sub (word.sub src0 (word.of_Z 1))(word.sub (word.sub n0 (word.of_Z 1)) (word.of_Z 1)))
+              with (word.sub src0 (word.sub n0 (word.of_Z 1))) by ZnWords.
+            eassumption. }
+          { replace (word.sub (word.sub dst0 (word.of_Z 1)) (word.sub (word.sub n0 (word.of_Z 1)) (word.of_Z 1)))
+              with (word.sub dst0 (word.sub n0 (word.of_Z 1))) by ZnWords.
+            eassumption. }
+          { ZnWords. }
+          { cbn in *; ZnWords. }
+          { cbn in *; ZnWords. }
+          { cbn in *; ZnWords. }
+          split.
+          { cbn in *; ZnWords. }
+          intuition idtac; repeat straightline_cleanup.
+          eapply map.split_put_r2l in H22; trivial.
+          rewrite map.of_list_word_at_snoc by ZnWords.
+          progress replace (word.add (word.sub dst0 (word.sub n0 (word.of_Z 1))) (word.of_Z (length s0))) with dst0 by ZnWords.
+          progress replace (word.sub (word.sub dst0 (word.of_Z 1)) (word.sub (word.sub n0 (word.of_Z 1)) (word.of_Z 1))) with (word.sub dst0 (word.sub n0 (word.of_Z 1))) in H22 by ZnWords.
+          exact H22. }
+        { cbn. intuition idtac. eexists _, _; ssplit; eauto. f_equal. ZnWords. } }
+  Qed.
+
+  Require Import coqutil.Macros.symmetry.
+  Local Notation "xs $@ a" := (Array.array ptsto (word.of_Z 1) a xs) (at level 10, format "xs $@ a").
+  Global Instance spec_of_memmove_array : spec_of "memmove" :=
+    fnspec! "memmove" (dst src n : word) / (d s : list byte) (R Rs : mem -> Prop),
+    { requires t m := m =* s$@src * Rs /\ m =* d$@dst * R /\
+        length s = n :> Z /\ length d = n :> Z /\ n <= 2^(width-1);
+      ensures t' m := m =* s$@dst * R /\ t=t' }.
+
+  Lemma memmove_ok_array : program_logic_goal_for_function! memmove.
+  Proof.
+    cbv [program_logic_goal_for spec_of_memmove_array]; intros.
+    eapply WeakestPreconditionProperties.Proper_call; cycle 1; [eapply memmove_ok|];
+        cbv [sepclause_of_map] in *.
+    { intuition idtac.
+      - seprewrite_in_by @ptsto_bytes.array1_iff_eq_of_list_word_at H0 ZnWords; eassumption.
+      - seprewrite_in_by @ptsto_bytes.array1_iff_eq_of_list_word_at H ZnWords; eassumption.
+      - trivial.
+      - trivial. }
+    { intros ? ? ? ?. intuition idtac.
+      seprewrite_in_by (symmetry! @ptsto_bytes.array1_iff_eq_of_list_word_at) H2 ZnWords; eassumption. }
+  Qed.
 End WithParameters.
